updates

intermediate/Veritas.Intermediate.Correctness.fst
@@ -1,16 +1,52 @@
 module Veritas.Intermediate.Correctness
 
+open Veritas.Hash
+open Veritas.Record
+open Veritas.SeqMachine
 open Veritas.State
+open Veritas.StateSeqMachine
 open Veritas.Verifier.EAC
 open Veritas.Intermediate.Global
 open Veritas.Intermediate.Thread
 open Veritas.Intermediate.VerifierConfig
 
+module I = Veritas.Interleave
 module IntG = Veritas.Intermediate.Global
+module IntTL = Veritas.Intermediate.TSLog
+
+
+let lemma_time_seq_rw_consistent  #vcfg
+  (il: IntTL.hash_verifiable_log vcfg {~ (rw_consistent (IntTL.to_state_ops il))})
+  : hash_collision_gen = admit()
 
 // final correctness property
 let lemma_verifier_correct (#vcfg:_) (gl: hash_verifiable_log vcfg { ~ (seq_consistent (IntG.to_state_ops gl))})
   : hash_collision_gen = 
   (* sequences of per-thread put/get operations *)
   let g_ops = IntG.to_state_ops gl in
-  admit()
+  
+  (* sequence ordered by time of each log entry *)
+  let il = IntTL.create gl in  
+  I.lemma_interleaving_correct il;
+  assert(I.interleave (I.i_seq il) gl);
+
+  (* sequence of state ops induced by tmsl *)
+  let ts_ops = IntTL.to_state_ops il in
+  IntTL.lemma_logS_interleave_implies_state_ops_interleave (I.i_seq il) gl;
+  assert(I.interleave ts_ops g_ops);
+
+  let is_rw_consistent = valid_all_comp ssm ts_ops in
+  lemma_state_sm_equiv_rw_consistent ts_ops;
+
+    if is_rw_consistent then (
+      assert(valid_all ssm ts_ops);
+      assert(rw_consistent ts_ops);
+
+      (* a contradiction *)
+      assert(seq_consistent g_ops);
+
+      (* any return value *)
+      SingleHashCollision (Collision (DVal Null) (DVal Null))
+    )
+    else
+      lemma_time_seq_rw_consistent il
