intermediate/Veritas.Intermediate.TSLog.fsti
@@ -5,7 +5,9 @@ open Veritas.State
 open Veritas.Intermediate.Global
 open Veritas.Intermediate.Logs
 
+module I = Veritas.Interleave
 module IntL = Veritas.Intermediate.Logs
+module IntG = Veritas.Intermediate.Global
 
 let il_logS vcfg = interleaving (logS_entry vcfg)
 
@@ -17,3 +19,30 @@ let g_logS_of #vcfg (il:il_logS vcfg): g_logS _ = s_seq il
 
 let to_state_ops #vcfg (itsl:il_logS vcfg): Seq.seq (state_op) =
   IntL.to_state_ops (i_seq itsl)
+
+let verifiable #vcfg (il: il_logS vcfg) = 
+  IntG.verifiable (g_logS_of il)
+
+val clock_sorted (#vcfg:_) (il: il_logS vcfg {verifiable il}): prop
+
+let its_log vcfg = il:il_logS vcfg{verifiable il /\ clock_sorted il}
+
+val create (#vcfg:_) (gl: verifiable_log vcfg): (itsl:its_log vcfg{g_logS_of itsl == gl})
+
+let hash_verifiable #vcfg (itsl: its_log vcfg) = IntG.hash_verifiable (g_logS_of itsl)
+
+let hash_verifiable_log vcfg = itsl: its_log vcfg{hash_verifiable itsl}
+
+val lemma_prefix_verifiable (#vcfg:_) (itsl: its_log vcfg) (i:nat{i <= I.length itsl}):
+  Lemma (ensures (verifiable (I.prefix itsl i) /\ clock_sorted (I.prefix itsl i)))
+        [SMTPat (I.prefix itsl i)]
+
+let lemma_logS_interleave_implies_state_ops_interleave #vcfg (l: logS vcfg) (gl: g_logS vcfg{interleave #(logS_entry vcfg) l gl})
+  : Lemma (interleave #state_op (IntL.to_state_ops l) (IntG.to_state_ops gl)) 
+  = FStar.Squash.bind_squash
+      #(interleave l gl)
+      #(interleave (IntL.to_state_ops l) (IntG.to_state_ops gl))
+      ()
+      (fun i -> 
+        let i' = filter_map_interleaving is_state_op to_state_op i in
+        FStar.Squash.return_squash i')
